Phi_System/PhiSem_Formalization_Tools.thy
@@ -50,8 +50,8 @@ lemma \<phi>M_assume[intro!]:
 lemma \<phi>M_tail_left:  \<open>\<p>\<r>\<o>\<c> F \<lbrace> 1\<heavy_comma> X \<longmapsto> Y \<rbrace> \<t>\<h>\<r>\<o>\<w>\<s> E \<Longrightarrow> \<p>\<r>\<o>\<c> F \<lbrace> X \<longmapsto> Y \<rbrace> \<t>\<h>\<r>\<o>\<w>\<s> E\<close> by simp
 lemma \<phi>M_tail_right: \<open>\<p>\<r>\<o>\<c> F \<lbrace> X \<longmapsto> \<lambda>v. 1 \<heavy_comma> Y v \<rbrace> \<t>\<h>\<r>\<o>\<w>\<s> E \<Longrightarrow> \<p>\<r>\<o>\<c> F \<lbrace> X \<longmapsto> Y \<rbrace> \<t>\<h>\<r>\<o>\<w>\<s> E\<close> by simp
 lemma \<phi>M_tail_right_right: \<open>\<p>\<r>\<o>\<c> F \<lbrace> X \<longmapsto> \<lambda>v. Y v\<heavy_comma> 1 \<rbrace> \<t>\<h>\<r>\<o>\<w>\<s> E \<Longrightarrow> \<p>\<r>\<o>\<c> F \<lbrace> X \<longmapsto> Y \<rbrace> \<t>\<h>\<r>\<o>\<w>\<s> E\<close> by simp
-lemma \<phi>M_detail_left[intro!]:  \<open>\<p>\<r>\<o>\<c> F \<lbrace> X \<longmapsto> Y \<rbrace> \<t>\<h>\<r>\<o>\<w>\<s> E \<Longrightarrow> \<p>\<r>\<o>\<c> F \<lbrace> 1\<heavy_comma> X \<longmapsto> Y \<rbrace> \<t>\<h>\<r>\<o>\<w>\<s> E\<close> by simp
-lemma \<phi>M_detail_right[intro!]: \<open>\<p>\<r>\<o>\<c> F \<lbrace> X \<longmapsto> Y \<rbrace> \<t>\<h>\<r>\<o>\<w>\<s> E \<Longrightarrow> \<p>\<r>\<o>\<c> F \<lbrace> X \<longmapsto> \<lambda>v. 1\<heavy_comma> Y v \<rbrace> \<t>\<h>\<r>\<o>\<w>\<s> E\<close> by simp
+lemma \<phi>M_shrink_left:  \<open>\<p>\<r>\<o>\<c> F \<lbrace> X \<longmapsto> Y \<rbrace> \<t>\<h>\<r>\<o>\<w>\<s> E \<Longrightarrow> \<p>\<r>\<o>\<c> F \<lbrace> 1\<heavy_comma> X \<longmapsto> Y \<rbrace> \<t>\<h>\<r>\<o>\<w>\<s> E\<close> by simp
+lemma \<phi>M_shrink_right[intro!]: \<open>\<p>\<r>\<o>\<c> F \<lbrace> X \<longmapsto> Y \<rbrace> \<t>\<h>\<r>\<o>\<w>\<s> E \<Longrightarrow> \<p>\<r>\<o>\<c> F \<lbrace> X \<longmapsto> \<lambda>v. 1\<heavy_comma> Y v \<rbrace> \<t>\<h>\<r>\<o>\<w>\<s> E\<close> by simp
 
 lemma \<phi>M_getV_raw[intro!]:
    \<open>(v \<in> (x \<Ztypecolon> A) \<Longrightarrow> \<p>\<r>\<o>\<c> F (VDT_dest v) \<lbrace> X \<longmapsto> Y \<rbrace> \<t>\<h>\<r>\<o>\<w>\<s> E  )
@@ -78,8 +78,17 @@ lemma \<phi>M_caseV[intro!]:
 
 subsection \<open>Elementary Constructions for Reasoning Fictions\<close>
 
-definition \<phi>Res_Spec :: \<open>rassn \<Rightarrow> rassn\<close>
+text \<open>It is a Hybrid Dynamic Logic\<close>
+
+ definition \<phi>Res_Spec :: \<open>rassn \<Rightarrow> rassn\<close>
   where \<open>\<phi>Res_Spec P = (RES.SPACE \<inter> P)\<close>
+(*
+term \<open><results>\<close>
+
+definition \<phi>Res_Sat  :: \<open>resource \<Rightarrow> rassn \<Rightarrow> bool\<close> ("\<s>\<t>\<a>\<t>\<e> _ \<i>\<s> _" [1000,11] 10)
+  where \<open>\<phi>Res_Sat s P \<longleftrightarrow> s \<in> \<phi>Res_Spec P\<close>
+
+definition \<phi>Comp_Sat :: \<open>\<close> *)
 
 lemma \<phi>Res_Spec_0[iff]:
   \<open>\<phi>Res_Spec {} = {}\<close>
