Phi_Test/PhiTest_All_Sem.thy
@@ -1,0 +1,12 @@
+theory PhiTest_All_Sem
+  imports Phi_Semantics.PhiSem_Aggregate_Array
+          Phi_Semantics.PhiSem_Aggregate_Tuple
+          Phi_Semantics.PhiSem_CF_Routine
+          Phi_Semantics.PhiSem_CF_Breakable
+          Phi_Semantics.PhiSem_Variable
+          Phi_Semantics.PhiSem_Int_ArbiPrec
+          Phi_Semantics.PhiSem_Machine_Integer
+          Phi_Semantics.PhiSem_Mem_OO
+begin
+
+end
